src/program_proof/pav/advrpc.v
@@ -1,4 +1,5 @@
-From Perennial.program_proof Require Import grove_prelude.
+From Perennial.program_proof.pav Require Import prelude.
+
 From Goose.github_com.mit_pdos.pav Require Import advrpc.
 
 Module Server.
