src/program_proof/pav/rpc.v
@@ -1,7 +1,8 @@
-From Perennial.program_proof Require Import grove_prelude.
+From Perennial.program_proof.pav Require Import prelude.
 From Goose.github_com.mit_pdos.pav Require Import kt.
 
-From Perennial.program_proof.pav Require Import auditor advrpc core cryptoffi serde server.
+From Perennial.program_proof.pav Require Import
+  auditor advrpc core cryptoffi serde server.
 
 Section specs.
 Context `{!heapGS Σ, !pavG Σ}.
