src/program_proof/pav/server.v
@@ -1,8 +1,9 @@
 From New.experiments Require Import glob.
-From Perennial.program_proof Require Import grove_prelude.
+From Perennial.program_proof.pav Require Import prelude.
 From Goose.github_com.mit_pdos.pav Require Import kt.
 
-From Perennial.program_proof.pav Require Import core cryptoffi cryptoutil serde merkle.
+From Perennial.program_proof.pav Require Import
+  core cryptoffi cryptoutil serde merkle.
 From Perennial.goose_lang.lib.rwlock Require Import rwlock_noncrash.
 
 Module userState.
